Parser/Lexer.thy
@@ -1,0 +1,33 @@
+theory Lexer
+  imports "../OperationalSemantics/Program_Model" 
+          "../Prelims/Result" 
+          "../Prelims/AST_Prelims"
+    
+begin
+
+abbreviation \<open>isnt_lbracket x \<equiv> (x \<noteq> CHR ''('')\<close>
+
+function
+  lexer :: \<open>string \<Rightarrow> AST\<close>
+where
+  \<open>lexer str = (
+    let 
+      tstr = trim str;
+      name = takeWhile isnt_lbracket tstr;
+      bargstr = dropWhile isnt_lbracket tstr;
+      argstr = butlast (tl bargstr)
+    in
+      Node name (map lexer (split argstr))
+  )\<close>
+  by auto
+termination apply standard
+  apply (rule wf_mlex[of \<open>{}\<close> length])
+  apply (auto simp del: split.simps)
+  apply (rule mlex_less)
+  subgoal for str xd
+    apply (cases str, simp)
+    apply (drule length_split, auto)
+    by (smt (verit, ccfv_SIG) One_nat_def diff_Suc_eq_diff_pred diff_is_0_eq' diff_less leD leI le_trans length_append_singleton length_dropWhile_le length_rev linordered_nonzero_semiring_class.zero_le_one zero_less_Suc)
+  .
+
+end
