Parser/Lexer_Code.thy
@@ -1,0 +1,6 @@
+theory Lexer_Code
+  imports Lexer
+      (*"HOL-Library.Code_Abstract_Char"*)
+begin
+
+end
