Parser/Parse.thy
@@ -1,0 +1,28 @@
+theory Parse   
+  imports Translator_Code
+
+  keywords "BIL" :: thy_decl
+       and "BIL_file" :: thy_load
+begin
+
+ML_file \<open>ml/common.ml\<close>
+ML_file \<open>ml/bil_adt_parser.ml\<close>
+
+text \<open>BIL Parse, adds commands to parse BIR from strings (with BIR) or from files (with BIR_file)\<close>
+
+ML \<open>
+
+val _ =
+    Outer_Syntax.local_theory
+      \<^command_keyword>\<open>BIL\<close>
+      "Generate a locale from a list of BIL instructions."
+      (Parse.name -- Parse.embedded >> uncurry bil_parser)
+
+val _ =
+    Outer_Syntax.command
+      \<^command_keyword>\<open>BIL_file\<close>
+      "Generate a locale from a BIL file."
+      (Parse.name -- Resources.parse_file >> (Toplevel.theory o uncurry bil_file_parser))
+\<close>
+
+end
