ml/BIL_Parser.thy
@@ -1,8 +1,0 @@
-theory BIL_Parser
-  imports Main
-begin
-
-
-
-
-end
